code/ecdsap256/Hacl.Impl.P256.PointAdd.fsti
@@ -5,71 +5,43 @@ open FStar.HyperStack
 module ST = FStar.HyperStack.ST
 
 open Lib.IntTypes
-open Hacl.Impl.P256.Arithmetics
-
 open Lib.Buffer
 
-(* open Spec.P256.Lemmas *)
 open Hacl.Spec.P256.Definition
 open Spec.P256
-open Hacl.Impl.SolinasReduction
 open Hacl.Spec.P256.MontgomeryMultiplication
-open Hacl.Impl.P.LowLevel 
-open Hacl.Impl.P256.MontgomeryMultiplication
-open Spec.P256
-open Hacl.Impl.P256.Math 
 
-open Hacl.Impl.P256.PointDouble
-
-open FStar.Tactics 
-open FStar.Tactics.Canon
-
-open FStar.Math.Lemmas
-
-open FStar.Mul
 
 #set-options "--z3rlimit 100"
 
 val point_add: #c: curve -> p: point c -> q: point c -> result: point c 
   -> tempBuffer: lbuffer uint64 (size 22 *! getCoordinateLenU64 c) -> 
    Stack unit (requires fun h -> 
+     let prime = getPrime c in 
      live h p /\ live h q /\ live h result /\ live h tempBuffer /\ 
      eq_or_disjoint q result /\ disjoint p q /\ disjoint p tempBuffer /\ 
-     disjoint q tempBuffer /\ disjoint p result /\ disjoint result tempBuffer /\  
-    (
-      let prime = getPrime c in 
-      let len = getCoordinateLenU64 c in 
+     disjoint q tempBuffer /\ disjoint p result /\ disjoint result tempBuffer /\ 
+     
+     point_x_as_nat c h p < prime /\ 
+     point_y_as_nat c h p < prime /\ 
+     point_z_as_nat c h p < prime /\
       
-      as_nat c h (gsub p (size 0) len) < prime /\ 
-      as_nat c h (gsub p len len) < prime /\ 
-      as_nat c h (gsub p (size 2 *! len) len) < prime /\
-      
-      as_nat c h (gsub q (size 0) len) < prime /\ 
-      as_nat c h (gsub q len len) < prime /\ 
-      as_nat c h (gsub q (size 2 *! len) len) < prime
-      )
+     point_x_as_nat c h q < prime /\ 
+     point_y_as_nat c h q < prime /\ 
+     point_z_as_nat c h q < prime
    )
    (ensures fun h0 _ h1 -> 
-     modifies (loc tempBuffer |+| loc result) h0 h1 /\ 
-     (
-       let len : size_t = getCoordinateLenU64 c in 
-       let prime = getPrime c in 
+     modifies (loc tempBuffer |+| loc result) h0 h1 /\ (
+     let prime = getPrime c in 
+    
+     let pX, pY, pZ = point_x_as_nat c h0 p, point_y_as_nat c h0 p, point_z_as_nat c h0 p in 
+     let qX, qY, qZ = point_x_as_nat c h0 q, point_y_as_nat c h0 q, point_z_as_nat c h0 q in 
+     let x3, y3, z3 = point_x_as_nat c h1 result, point_y_as_nat c h1 result, point_z_as_nat c h1 result in 
      
-       as_nat c h1 (gsub result (size 0) len) < prime /\ 
-       as_nat c h1 (gsub result len len) < prime /\ 
-       as_nat c h1 (gsub result (2ul *! len) len) < prime /\
-       
-       (
-       let pX, pY, pZ = gsub p (size 0) len, gsub p len len, gsub p (size 2 *! len) len in 
-       let qX, qY, qZ = gsub q (size 0) len, gsub q len len, gsub q (size 2 *! len) len in 
-       let x3, y3, z3 = gsub result (size 0) len, gsub result len len, gsub result (size 2 *! len) len in 
-       
-       let pxD, pyD, pzD = fromDomain_ #c (as_nat c h0 pX), fromDomain_ #c (as_nat c h0 pY), fromDomain_ #c (as_nat c h0 pZ) in 
-       let qxD, qyD, qzD = fromDomain_ #c (as_nat c h0 qX), fromDomain_ #c (as_nat c h0 qY), fromDomain_ #c (as_nat c h0 qZ) in 
-       let x3D, y3D, z3D = fromDomain_ #c (as_nat c h1 x3), fromDomain_ #c (as_nat c h1 y3), fromDomain_ #c (as_nat c h1 z3) in
+     let pxD, pyD, pzD = fromDomain_ #c pX, fromDomain_ #c pY, fromDomain_ #c pZ in 
+     let qxD, qyD, qzD = fromDomain_ #c qX, fromDomain_ #c qY, fromDomain_ #c qZ in 
+     let x3D, y3D, z3D = fromDomain_ #c x3, fromDomain_ #c y3, fromDomain_ #c z3 in
       
-       let xN, yN, zN = _point_add #c (pxD, pyD, pzD) (qxD, qyD, qzD) in 
-       x3D == xN /\ y3D == yN /\ z3D == zN
-   )
-   )
-   )
+     let xN, yN, zN = _point_add #c (pxD, pyD, pzD) (qxD, qyD, qzD) in 
+
+     x3 < prime /\  y3 < prime /\ z3 < prime /\  x3D == xN /\ y3D == yN /\ z3D == zN))
